extraction/theories/ExtractionCorrectness.v
@@ -6,6 +6,7 @@ From ConCert.Extraction Require Import ExAst.
 From ConCert.Extraction Require Import Extraction.
 From ConCert.Extraction Require Import Optimize.
 From ConCert.Extraction Require Import OptimizeCorrectness.
+From ConCert.Extraction Require Import Transform.
 From ConCert.Extraction Require Import ResultMonad.
 From ConCert.Extraction Require Import WcbvEvalAux.
 From Coq Require Import Arith.
@@ -35,30 +36,6 @@ Module E := EAst.
 
 Notation "Σ 'p⊢' s ▷ t" := (PCUICWcbvEval.eval Σ s t) (at level 50, s, t at next level) : type_scope.
 
-Lemma eval_const_construct_mask {wfl:WcbvFlags} Σ kn ind c im cm :
-  trans_env Σ e⊢ E.tConst kn ▷ E.tConstruct ind c ->
-  valid_masks_env im cm Σ ->
-  get_const_mask cm kn = [].
-Proof.
-  intros ev valid.
-  depelim ev.
-  eapply valid_dearg_mask_constant in valid; eauto.
-  enough (#|get_const_mask cm kn| = 0) by (now destruct get_const_mask).
-  apply valid_dearg_mask_spec in valid as (Γ & inner & <- & <-).
-  clear -ev.
-  induction #|Γ| as [|Γlen IH] eqn:eq in Γ, inner, ev |- *.
-  - now destruct Γ.
-  - destruct Γ as [|[na [body|]] Γ]; cbn in *.
-    + easy.
-    + depelim ev.
-      refold.
-      rewrite subst_it_mkLambda_or_LetIn in ev2.
-      erewrite <- vasses_subst_context.
-      eapply IH; [eassumption|].
-      now rewrite length_subst_context.
-    + depelim ev.
-Qed.
-
 Lemma wf_squash {Σ} :
   ∥wf_ext Σ∥ ->
   ∥wf Σ∥.
@@ -77,7 +54,7 @@ Proof.
 Qed.
 
 Theorem extract_correct
-        (wfl := default_wcbv_flags)
+        (wfl := opt_wcbv_flags)
         (Σ : P.global_env_ext) (wfΣ : ∥wf_ext Σ∥)
         kn ui ind c ui' ignored exΣ :
   axiom_free Σ ->
@@ -91,15 +68,14 @@ Theorem extract_correct
   ∥trans_env exΣ e⊢ E.tConst kn ▷ E.tConstruct ind c∥.
 Proof.
   intros ax [T wt] ev not_erasable no_ignores ex.
-  cbn in *.
-  destruct env_closed eqn:closed; cbn in *; [|congruence].
-  destruct analyze_env eqn:an; cbn in *.
-  destruct is_expanded_env eqn:isexp; cbn in *; [|congruence].
-  destruct valid_masks_env eqn:valid; cbn in *; [|congruence].
-  inversion_clear ex.
+  cbn -[dearg_transform] in *.
+  destruct dearg_transform eqn:dt; cbn -[dearg_transform] in *; [|congruence].
+  injection ex as ->.
   destruct wfΣ.
-  eapply erases_correct in ev as (erv& erase_to & [erev]); eauto.
+  eapply erases_correct in ev as (erv&erase_to&[erev]).
   2: constructor; auto.
+  2: eassumption.
+  2: apply erases_tConst.
   2: { eapply inversion_Const in wt as (?&?&?&?&?); auto.
        eapply global_erased_with_deps_erases_deps_tConst; eauto.
        eapply (erase_global_decls_deps_recursive_correct
@@ -109,22 +85,12 @@ Proof.
          unfold declared_constant, PCUICAst.fst_ctx, fst_ctx in *.
          congruence.
        - now apply KernameSet.singleton_spec. }
-
   depelim erase_to; [|easy].
-  eapply eval_const_construct_mask in erev as no_mask; eauto.
-  assert (ctor_exp := erev).
-  eapply eval_is_expanded_aux with (k := 0) in ctor_exp; eauto.
-  2: now cbn; rewrite no_mask.
-  cbn in *.
-  eapply dearg_correct in erev; eauto.
-  - cbn in *.
-    rewrite no_mask in erev.
-    destruct get_ctor_mask; [|easy].
-    cbn in *.
-    constructor.
-    now apply eval_debox_env_types.
-  - cbn.
-    now rewrite no_mask.
+
+  constructor.
+  eapply dearg_transform_correct; eauto.
+  apply (OptimizePropDiscr.optimize_correct _ (tConst kn) (tConstruct ind c)).
+  assumption.
 Qed.
 
 Print Assumptions extract_correct.
